Prove order strengthening (#76)

src/lang/Event.v
@@ -105,4 +105,37 @@ Module ProgramEvent.
     | update loc _ _ _ ordw => Some (loc, ordw)
     | _ => None
     end.
+
+  Inductive ord: forall (e1 e2:t), Prop :=
+  | ord_read
+      l v o1 o2
+      (O: Ordering.le o1 o2):
+      ord (read l v o1) (read l v o2)
+  | ord_write
+      l v o1 o2
+      (O: Ordering.le o1 o2):
+      ord (write l v o1) (write l v o2)
+  | ord_update
+      l vr vw or1 or2 ow1 ow2
+      (OR: Ordering.le or1 or2)
+      (OW: Ordering.le ow1 ow2):
+      ord (update l vr vw or1 ow1) (update l vr vw or2 ow2)
+  | ord_fence
+      or1 or2 ow1 ow2
+      (OR: Ordering.le or1 or2)
+      (OW: Ordering.le ow1 ow2):
+      ord (fence or1 ow1) (fence or2 ow2)
+  | ord_syscall
+      e:
+      ord (syscall e) (syscall e)
+  .
+
+  Inductive ord_opt: forall (e1 e2:option t), Prop :=
+  | ord_opt_none:
+      ord_opt None None
+  | ord_opt_some
+      e1 e2
+      (ORD: ord e1 e2):
+      ord_opt (Some e1) (Some e2)
+  .
 End ProgramEvent.
